Sep_Log_Frag.thy
@@ -1,4 +1,7 @@
 theory Sep_Log_Frag 
 imports "decision_procedure/Proof_System"
 begin
+
+(* The whole session can be build and generates a PDF with a short abstract as introduction. *)
+
 end
