decision_procedure/Proof_System.thy
@@ -71,6 +71,7 @@ qed
 theorem non_empty_ls: "E\<^sub>1\<noteq>\<^sub>pE\<^sub>3 \<and>\<^sub>p \<Pi>\<bar>\<Sigma> \<turnstile> \<Pi>'\<bar>ls(E\<^sub>2,E\<^sub>3) * \<Sigma>' 
   \<Longrightarrow> E\<^sub>1\<noteq>\<^sub>pE\<^sub>3 \<and>\<^sub>p \<Pi>\<bar>E\<^sub>1\<longmapsto>E\<^sub>2 * \<Sigma> \<turnstile> \<Pi>'\<bar>ls(E\<^sub>1,E\<^sub>3) * \<Sigma>'"
 proof (rule entailment_lift)
+  define xs where xs: "xs = -(fv E\<^sub>1 \<union> fv E\<^sub>2 \<union> fv E\<^sub>3)"
   fix s h
   assume assm1: "E\<^sub>1\<noteq>\<^sub>pE\<^sub>3 \<and>\<^sub>p \<Pi>\<bar>\<Sigma> \<turnstile> \<Pi>'\<bar>ls(E\<^sub>2,E\<^sub>3) * \<Sigma>'"
   assume assm2: "(s,h)\<Turnstile>E\<^sub>1\<noteq>\<^sub>pE\<^sub>3 \<and>\<^sub>p \<Pi>\<bar>E\<^sub>1\<longmapsto>E\<^sub>2 * \<Sigma>"
@@ -88,20 +89,21 @@ proof (rule entailment_lift)
     "(s,h2_2)\<Turnstile>SpatF \<Sigma>'" by blast
   then obtain m where tail: "(s,h2_1)\<Turnstile>ls\<^sup>m(E\<^sub>2,E\<^sub>3)" by fast
   then obtain n where n: "n = Suc m" by simp
-  obtain x where "x \<notin> fv E\<^sub>1 \<union> fv E\<^sub>2 \<union> fv E\<^sub>3" using fv_finite_expr fv_finite_un fv_other_x_un
-    by (metis Un_iff fv_expr.elims singleton_iff)
-  {
-    hence "x \<notin> fv E\<^sub>2 \<union> fv E\<^sub>3" by fast
+  have "\<forall>x \<in> xs. (s(x:=\<lbrakk>E\<^sub>2\<rbrakk>s),h2_1)\<Turnstile>ls\<^sup>m(\<acute>x`,E\<^sub>3)"
+  proof
+    fix x
+    assume "x \<in> xs"
+    with xs have "x \<notin> fv E\<^sub>2 \<union> fv E\<^sub>3" by fast
     from ls_extend_rhs[OF tail this] have tail_ext: "(s(x:=\<lbrakk>E\<^sub>2\<rbrakk>s),h2_1)\<Turnstile>ls\<^sup>m(E\<^sub>2,E\<^sub>3)" .
     have "\<lbrakk>E\<^sub>2\<rbrakk>s(x:=\<lbrakk>E\<^sub>2\<rbrakk>s) = \<lbrakk>\<acute>x`\<rbrakk>s(x:=\<lbrakk>E\<^sub>2\<rbrakk>s)"
       by (metis eval.simps(1) eval.simps(2) expr.exhaust fun_upd_apply)
-    from ls_change_fst_general[OF tail_ext this] have "(s(x:=\<lbrakk>E\<^sub>2\<rbrakk>s),h2_1)\<Turnstile>ls\<^sup>m(\<acute>x`,E\<^sub>3)" .
-  }
-  from \<open>x \<notin> fv E\<^sub>1 \<union> fv E\<^sub>2 \<union> fv E\<^sub>3\<close> have "x \<notin> fv E\<^sub>1 \<union> fv E\<^sub>3" by simp
+    from ls_change_fst[OF tail_ext this] show "(s(x:=\<lbrakk>E\<^sub>2\<rbrakk>s),h2_1)\<Turnstile>ls\<^sup>m(\<acute>x`,E\<^sub>3)" .
+  qed
   from sep_conj sep_conj2 have "h1\<bottom>h2_1" by auto
+  from xs have "xs \<subseteq> -(fv E\<^sub>1 \<union> fv E\<^sub>3)" by blast
   have "h1++h2_1=h1++h2_1" by simp
-  from ListSegment[OF hd \<open>x \<notin> fv E\<^sub>1 \<union> fv E\<^sub>3\<close> \<open>h1\<bottom>h2_1\<close> this \<open>(s(x:=\<lbrakk>E\<^sub>2\<rbrakk>s),h2_1)\<Turnstile>ls\<^sup>m(\<acute>x`,E\<^sub>3)\<close> n 
-    \<open>\<lbrakk>E\<^sub>1\<rbrakk>s\<noteq>\<lbrakk>E\<^sub>3\<rbrakk>s\<close>] have "(s,h1++h2_1)\<Turnstile>ls\<^sup>n(E\<^sub>1,E\<^sub>3)" .
+  from ListSegment[OF hd \<open>xs \<subseteq> -(fv E\<^sub>1 \<union> fv E\<^sub>3)\<close> \<open>\<forall>x \<in> xs. (s(x:=\<lbrakk>E\<^sub>2\<rbrakk>s),h2_1)\<Turnstile>ls\<^sup>m(\<acute>x`,E\<^sub>3)\<close> \<open>h1\<bottom>h2_1\<close>
+    this n \<open>\<lbrakk>E\<^sub>1\<rbrakk>s\<noteq>\<lbrakk>E\<^sub>3\<rbrakk>s\<close>] have "(s,h1++h2_1)\<Turnstile>ls\<^sup>n(E\<^sub>1,E\<^sub>3)" .
   {
     hence "(s,h1++h2_1)\<Turnstile>Spat (ls(E\<^sub>1,E\<^sub>3))" by auto
     moreover from sep_conj(1,2) sep_conj2(1,2) have "h=h1++h2_1++h2_2" "h1++h2_1\<bottom>h2_2" by auto
